bloom-filter/Spec.BloomFilter.fst
@@ -18,7 +18,7 @@ assume val hash: element -> u32
 type count = n:nat
 
 let contains (#a:eqtype) (l:list (a & count)) (e:a) : Tot bool =
-  existsb (fun (e', _) -> e = e') l
+  existsb (fun ((e', n) : a & count) -> e = e' && n > 0) l
 
 let rec no_duplicates (#a:eqtype) (l:list (a & count)) : Tot bool (decreases l) =
   match l with
@@ -53,103 +53,31 @@ let rec element_count #a l e = match l with
   | (e', count)::tl ->
     if e = e' then count else element_count tl e
 
+let same_elements_except (#a:eqtype) (l1 l2: count_list a) (e:a) =
+   (forall (e':a{e' <> e}). contains l1 e' <==> contains l2 e')
+
 val decr_count:
   #a:eqtype ->
   l:count_list a ->
   e : a{contains l e} ->
   Tot (l':count_list a{
-      same_elements l l'
+      if element_count l e > 1 then
+        same_elements l l'
+      else
+        same_elements_except l l' e /\ not (contains l' e)
   }) (decreases l)
 let rec decr_count #a l e =
   match l with
   | [] -> l
   | (e', old_count)::tl ->
     if e = e' then
-      if old_count = 0 then
-      (* We saturate at 0 *)
-        (e', old_count)::tl
-      else
-        (e', old_count - 1)::tl
+      (e', old_count - 1)::tl
     else
       (e', old_count)::(decr_count tl e)
 
 type spec_bloom_storage_u8 = {
    elements: (l:(count_list element){no_duplicates l})
 }
-
-let rec all_elements
-  (#a:eqtype)
-  (l:count_list a)
-  (f:a -> bool)
-  : Tot (b:bool) (decreases l) =
-  match l with
-  | [] -> true
-  | (hd,_)::tl -> if f hd then all_elements tl f else false
-
-let rec all_elements_lemma1
-  (#a:eqtype)
-  (l: count_list a)
-  (f:a -> bool)
-  : Lemma (ensures (
-    all_elements #a l f ==>
-      (forall (e:a{contains l e}). f e)
-    )) (decreases l)
-  =
-  if not (all_elements #a l f) then () else
-  match l with
-  | [] -> ()
-  | (e_hd,_)::tl ->
-    assert (not (contains tl e_hd));
-    if not (f e_hd) then assert(false) else begin
-      let inner_lemma
-	(e:a{contains l e})
-	: Lemma (ensures (f e)) =
-	assert (e = e_hd \/ contains tl e);
-	Classical.or_elim
-	  #(e = e_hd)
-	  #(contains tl e)
-	  #(fun _ -> f e)
-	  (fun _ -> assert (e = e_hd))
-	  (fun _ -> assert (contains tl e);
-	    all_elements_lemma1 #a tl f
-	  )
-      in
-      Classical.forall_intro inner_lemma
-    end
-
-let rec all_elements_lemma2
-  (#a:eqtype)
-  (l: count_list a)
-  (f:a -> bool)
-  : Lemma (ensures (
-    (forall (e:a{contains l e}). f e) ==>
-      all_elements #a l f
-    )) (decreases l)
-  =
-  let rec inner_lemma
-    (_ : (forall (e:a{contains l e}). f e))
-    : Lemma (ensures (all_elements #a l f))
-    = match l with
-    | [] -> ()
-    | (hd, _)::tl -> all_elements_lemma2 #a tl f
-  in
-  Classical.impl_intro
-    #((forall (e:a{contains l e}). f e))
-    #(all_elements #a l f)
-    inner_lemma
-
-
-let rec all_elements_lemma
-  (#a:eqtype)
-  (l: count_list a)
-  (f:a -> bool)
-  : Lemma (ensures (
-    all_elements #a l f <==>
-      (forall (e:a{contains l e}). f e)
-    )) (decreases l)
-  =
-  all_elements_lemma1 #a l f;
-  all_elements_lemma2 #a l f
 
 val spec_insert_element:
   bf:spec_bloom_storage_u8 ->
@@ -175,19 +103,20 @@ let lemma_spec_insert_element
 
 val spec_remove_element:
   bf:spec_bloom_storage_u8 ->
-  e:element ->
+  e:element{contains bf.elements e} ->
   Tot spec_bloom_storage_u8
 let spec_remove_element bf e =
-  if contains bf.elements e  then
     { bf with elements = decr_count bf.elements e }
-  else
-    bf
 
 let lemma_spec_remove_element
   (bf:spec_bloom_storage_u8)
-  (e:element)
+  (e:element{contains bf.elements e})
   : Lemma (ensures (
     let new_bf = spec_remove_element bf e in
-    same_elements bf.elements new_bf.elements
+    if element_count bf.elements e > 1 then
+      same_elements bf.elements new_bf.elements
+    else
+      same_elements_except bf.elements new_bf.elements e /\
+      not (contains new_bf.elements e)
   )) =
   ()
